Semantics/TreeToGraphThms.thy
@@ -11,95 +11,95 @@ Hopefully these shouldn't really be required.
 
 lemma mono_abs:
   assumes "kind g1 n = AbsNode x \<and> kind g2 n = AbsNode x"
-  assumes "(g1 \<turnstile> x \<triangleright> xe1) \<and> (g2 \<turnstile> x \<triangleright> xe2)"
-  assumes "xe1 \<le> xe2"
-  assumes "(g1 \<turnstile> n \<triangleright> e1) \<and> (g2 \<turnstile> n \<triangleright> e2)"
-  shows "e1 \<le> e2"
+  assumes "(g1 \<turnstile> x \<simeq> xe1) \<and> (g2 \<turnstile> x \<simeq> xe2)"
+  assumes "xe1 \<ge> xe2"
+  assumes "(g1 \<turnstile> n \<simeq> e1) \<and> (g2 \<turnstile> n \<simeq> e2)"
+  shows "e1 \<ge> e2"
   by (metis AbsNode assms(1) assms(2) assms(3) assms(4) mono_unary repDet)
 
 lemma mono_not:
   assumes "kind g1 n = NotNode x \<and> kind g2 n = NotNode x"
-  assumes "(g1 \<turnstile> x \<triangleright> xe1) \<and> (g2 \<turnstile> x \<triangleright> xe2)"
-  assumes "xe1 \<le> xe2"
-  assumes "(g1 \<turnstile> n \<triangleright> e1) \<and> (g2 \<turnstile> n \<triangleright> e2)"
-  shows "e1 \<le> e2"
+  assumes "(g1 \<turnstile> x \<simeq> xe1) \<and> (g2 \<turnstile> x \<simeq> xe2)"
+  assumes "xe1 \<ge> xe2"
+  assumes "(g1 \<turnstile> n \<simeq> e1) \<and> (g2 \<turnstile> n \<simeq> e2)"
+  shows "e1 \<ge> e2"
   by (metis NotNode assms(1) assms(2) assms(3) assms(4) mono_unary repDet)
 
 lemma mono_negate:
   assumes "kind g1 n = NegateNode x \<and> kind g2 n = NegateNode x"
-  assumes "(g1 \<turnstile> x \<triangleright> xe1) \<and> (g2 \<turnstile> x \<triangleright> xe2)"
-  assumes "xe1 \<le> xe2"
-  assumes "(g1 \<turnstile> n \<triangleright> e1) \<and> (g2 \<turnstile> n \<triangleright> e2)"
-  shows "e1 \<le> e2"
+  assumes "(g1 \<turnstile> x \<simeq> xe1) \<and> (g2 \<turnstile> x \<simeq> xe2)"
+  assumes "xe1 \<ge> xe2"
+  assumes "(g1 \<turnstile> n \<simeq> e1) \<and> (g2 \<turnstile> n \<simeq> e2)"
+  shows "e1 \<ge> e2"
   by (metis NegateNode assms(1) assms(2) assms(3) assms(4) mono_unary repDet)
 
 lemma mono_logic_negation:
   assumes "kind g1 n = LogicNegationNode x \<and> kind g2 n = LogicNegationNode x"
-  assumes "(g1 \<turnstile> x \<triangleright> xe1) \<and> (g2 \<turnstile> x \<triangleright> xe2)"
-  assumes "xe1 \<le> xe2"
-  assumes "(g1 \<turnstile> n \<triangleright> e1) \<and> (g2 \<turnstile> n \<triangleright> e2)"
-  shows "e1 \<le> e2"
+  assumes "(g1 \<turnstile> x \<simeq> xe1) \<and> (g2 \<turnstile> x \<simeq> xe2)"
+  assumes "xe1 \<ge> xe2"
+  assumes "(g1 \<turnstile> n \<simeq> e1) \<and> (g2 \<turnstile> n \<simeq> e2)"
+  shows "e1 \<ge> e2"
   by (metis LogicNegationNode assms(1) assms(2) assms(3) assms(4) mono_unary repDet)
 
 lemma mono_narrow:
   assumes "kind g1 n = NarrowNode ib rb x \<and> kind g2 n = NarrowNode ib rb x"
-  assumes "(g1 \<turnstile> x \<triangleright> xe1) \<and> (g2 \<turnstile> x \<triangleright> xe2)"
-  assumes "xe1 \<le> xe2"
-  assumes "(g1 \<turnstile> n \<triangleright> e1) \<and> (g2 \<turnstile> n \<triangleright> e2)"
-  shows "e1 \<le> e2"
+  assumes "(g1 \<turnstile> x \<simeq> xe1) \<and> (g2 \<turnstile> x \<simeq> xe2)"
+  assumes "xe1 \<ge> xe2"
+  assumes "(g1 \<turnstile> n \<simeq> e1) \<and> (g2 \<turnstile> n \<simeq> e2)"
+  shows "e1 \<ge> e2"
   using assms mono_unary repDet NarrowNode
   by metis
 
 lemma mono_sign_extend:
   assumes "kind g1 n = SignExtendNode ib rb x \<and> kind g2 n = SignExtendNode ib rb x"
-  assumes "(g1 \<turnstile> x \<triangleright> xe1) \<and> (g2 \<turnstile> x \<triangleright> xe2)"
-  assumes "xe1 \<le> xe2"
-  assumes "(g1 \<turnstile> n \<triangleright> e1) \<and> (g2 \<turnstile> n \<triangleright> e2)"
-  shows "e1 \<le> e2"
+  assumes "(g1 \<turnstile> x \<simeq> xe1) \<and> (g2 \<turnstile> x \<simeq> xe2)"
+  assumes "xe1 \<ge> xe2"
+  assumes "(g1 \<turnstile> n \<simeq> e1) \<and> (g2 \<turnstile> n \<simeq> e2)"
+  shows "e1 \<ge> e2"
   by (metis SignExtendNode assms(1) assms(2) assms(3) assms(4) mono_unary repDet)
 
 lemma mono_zero_extend:
   assumes "kind g1 n = ZeroExtendNode ib rb x \<and> kind g2 n = ZeroExtendNode ib rb x"
-  assumes "(g1 \<turnstile> x \<triangleright> xe1) \<and> (g2 \<turnstile> x \<triangleright> xe2)"
-  assumes "xe1 \<le> xe2"
-  assumes "(g1 \<turnstile> n \<triangleright> e1) \<and> (g2 \<turnstile> n \<triangleright> e2)"
-  shows "e1 \<le> e2"
+  assumes "(g1 \<turnstile> x \<simeq> xe1) \<and> (g2 \<turnstile> x \<simeq> xe2)"
+  assumes "xe1 \<ge> xe2"
+  assumes "(g1 \<turnstile> n \<simeq> e1) \<and> (g2 \<turnstile> n \<simeq> e2)"
+  shows "e1 \<ge> e2"
   using assms mono_unary repDet ZeroExtendNode
   by metis
 
 lemma mono_conditional:
   assumes "kind g1 n = ConditionalNode c t f \<and> kind g2 n = ConditionalNode c t f"
-  assumes "(g1 \<turnstile> c \<triangleright> ce1) \<and> (g2 \<turnstile> c \<triangleright> ce2)"
-  assumes "(g1 \<turnstile> t \<triangleright> te1) \<and> (g2 \<turnstile> t \<triangleright> te2)"
-  assumes "(g1 \<turnstile> f \<triangleright> fe1) \<and> (g2 \<turnstile> f \<triangleright> fe2)"
-  assumes "ce1 \<le> ce2 \<and> te1 \<le> te2 \<and> fe1 \<le> fe2"
-  assumes "(g1 \<turnstile> n \<triangleright> e1) \<and> (g2 \<turnstile> n \<triangleright> e2)"
-  shows "e1 \<le> e2"
+  assumes "(g1 \<turnstile> c \<simeq> ce1) \<and> (g2 \<turnstile> c \<simeq> ce2)"
+  assumes "(g1 \<turnstile> t \<simeq> te1) \<and> (g2 \<turnstile> t \<simeq> te2)"
+  assumes "(g1 \<turnstile> f \<simeq> fe1) \<and> (g2 \<turnstile> f \<simeq> fe2)"
+  assumes "ce1 \<ge> ce2 \<and> te1 \<ge> te2 \<and> fe1 \<ge> fe2"
+  assumes "(g1 \<turnstile> n \<simeq> e1) \<and> (g2 \<turnstile> n \<simeq> e2)"
+  shows "e1 \<ge> e2"
   by (metis ConditionalNodeE IRNode.inject(6) assms(1) assms(2) assms(3) assms(4) assms(5) assms(6) mono_conditional repDet rep_conditional)
 
 lemma mono_add:
   assumes "kind g1 n = AddNode x y \<and> kind g2 n = AddNode x y"
-  assumes "(g1 \<turnstile> x \<triangleright> xe1) \<and> (g2 \<turnstile> x \<triangleright> xe2)"
-  assumes "(g1 \<turnstile> y \<triangleright> ye1) \<and> (g2 \<turnstile> y \<triangleright> ye2)"
-  assumes "xe1 \<le> xe2 \<and> ye1 \<le> ye2"
-  assumes "(g1 \<turnstile> n \<triangleright> e1) \<and> (g2 \<turnstile> n \<triangleright> e2)"
-  shows "e1 \<le> e2"
+  assumes "(g1 \<turnstile> x \<simeq> xe1) \<and> (g2 \<turnstile> x \<simeq> xe2)"
+  assumes "(g1 \<turnstile> y \<simeq> ye1) \<and> (g2 \<turnstile> y \<simeq> ye2)"
+  assumes "xe1 \<ge> xe2 \<and> ye1 \<ge> ye2"
+  assumes "(g1 \<turnstile> n \<simeq> e1) \<and> (g2 \<turnstile> n \<simeq> e2)"
+  shows "e1 \<ge> e2"
   using mono_binary assms
   by (metis AddNodeE IRNode.inject(2) repDet rep_add)
 
 lemma mono_mul:
   assumes "kind g1 n = MulNode x y \<and> kind g2 n = MulNode x y"
-  assumes "(g1 \<turnstile> x \<triangleright> xe1) \<and> (g2 \<turnstile> x \<triangleright> xe2)"
-  assumes "(g1 \<turnstile> y \<triangleright> ye1) \<and> (g2 \<turnstile> y \<triangleright> ye2)"
-  assumes "xe1 \<le> xe2 \<and> ye1 \<le> ye2"
-  assumes "(g1 \<turnstile> n \<triangleright> e1) \<and> (g2 \<turnstile> n \<triangleright> e2)"
-  shows "e1 \<le> e2"
+  assumes "(g1 \<turnstile> x \<simeq> xe1) \<and> (g2 \<turnstile> x \<simeq> xe2)"
+  assumes "(g1 \<turnstile> y \<simeq> ye1) \<and> (g2 \<turnstile> y \<simeq> ye2)"
+  assumes "xe1 \<ge> xe2 \<and> ye1 \<ge> ye2"
+  assumes "(g1 \<turnstile> n \<simeq> e1) \<and> (g2 \<turnstile> n \<simeq> e2)"
+  shows "e1 \<ge> e2"
   using mono_binary assms
   by (metis IRNode.inject(26) MulNodeE repDet rep_mul)
 
 
 lemma encodes_contains:
-  assumes "g \<turnstile> n \<triangleright> e"
+  assumes "g \<turnstile> n \<simeq> e"
   shows "kind g n \<noteq> NoNode"
   using assms apply (induction rule: rep.induct)
   apply (metis IRNode.disc(349) is_ConstantNode_def)
@@ -125,7 +125,7 @@ lemma encodes_contains:
 
 lemma no_encoding:
   assumes "n \<notin> ids g"
-  shows "\<not>(g \<turnstile> n \<triangleright> e)"
+  shows "\<not>(g \<turnstile> n \<simeq> e)"
   using assms apply simp apply (rule notI) by (induction e; simp add: encodes_contains)
 
 lemma not_excluded_keep_type:
@@ -137,23 +137,23 @@ lemma not_excluded_keep_type:
 
 
 lemma graph_semantics_preservation:
-  assumes a: "e1' \<le> e2'"
+  assumes a: "e1' \<ge> e2'"
   assumes b: "({n'} \<unlhd> as_set g1) \<subseteq> as_set g2"
-  assumes c: "g1 \<turnstile> n' \<triangleright> e1'"
-  assumes d: "g2 \<turnstile> n' \<triangleright> e2'"
+  assumes c: "g1 \<turnstile> n' \<simeq> e1'"
+  assumes d: "g2 \<turnstile> n' \<simeq> e2'"
   shows "graph_refinement g1 g2"
   unfolding graph_refinement_def 
   apply (rule allI) apply (rule impI) apply (rule allI) apply (rule impI)
 proof -
   fix n e1
   assume e: "n \<in> ids g1"
-  assume f: "(g1 \<turnstile> n \<triangleright> e1)"
+  assume f: "(g1 \<turnstile> n \<simeq> e1)"
 
-  show "\<exists> e2. (g2 \<turnstile> n \<triangleright> e2) \<and> e1 \<le> e2"
+  show "\<exists> e2. (g2 \<turnstile> n \<simeq> e2) \<and> e1 \<ge> e2"
   proof (cases "n = n'")
     case True
     have g: "e1 = e1'" using c f True repDet by simp
-    have h: "(g2 \<turnstile> n \<triangleright> e2') \<and> e1' \<le> e2'"
+    have h: "(g2 \<turnstile> n \<simeq> e2') \<and> e1' \<ge> e2'"
       using True a d by blast
     then show ?thesis 
       using g by blast
@@ -175,32 +175,32 @@ proof -
         by (metis eq_refl rep.ParameterNode)
     next
       case (ConditionalNode n c t f ce1 te1 fe1)
-      have k: "g1 \<turnstile> n \<triangleright> ConditionalExpr ce1 te1 fe1" using f ConditionalNode
+      have k: "g1 \<turnstile> n \<simeq> ConditionalExpr ce1 te1 fe1" using f ConditionalNode
         by (simp add: ConditionalNode.hyps(2) rep.ConditionalNode)
       obtain cn tn fn where l: "kind g1 n = ConditionalNode cn tn fn"
         using ConditionalNode.hyps(1) by blast
-      then have mc: "g1 \<turnstile> cn \<triangleright> ce1"
+      then have mc: "g1 \<turnstile> cn \<simeq> ce1"
         using ConditionalNode.hyps(1) ConditionalNode.hyps(2) by fastforce
-      from l have mt: "g1 \<turnstile> tn \<triangleright> te1"
+      from l have mt: "g1 \<turnstile> tn \<simeq> te1"
         using ConditionalNode.hyps(1) ConditionalNode.hyps(3) by fastforce
-      from l have mf: "g1 \<turnstile> fn \<triangleright> fe1"
+      from l have mf: "g1 \<turnstile> fn \<simeq> fe1"
         using ConditionalNode.hyps(1) ConditionalNode.hyps(4) by fastforce
       then show ?case
       proof -
-        have "g1 \<turnstile> cn \<triangleright> ce1" using mc by simp
-        have "g1 \<turnstile> tn \<triangleright> te1" using mt by simp
-        have "g1 \<turnstile> fn \<triangleright> fe1" using mf by simp
-        have cer: "\<exists> ce2. (g2 \<turnstile> cn \<triangleright> ce2) \<and> ce1 \<le> ce2"
+        have "g1 \<turnstile> cn \<simeq> ce1" using mc by simp
+        have "g1 \<turnstile> tn \<simeq> te1" using mt by simp
+        have "g1 \<turnstile> fn \<simeq> fe1" using mf by simp
+        have cer: "\<exists> ce2. (g2 \<turnstile> cn \<simeq> ce2) \<and> ce1 \<ge> ce2"
           using ConditionalNode
           using a b c d l no_encoding not_excluded_keep_type repDet singletonD
           by (metis IRNode.inject(6))
-        have ter: "\<exists> te2. (g2 \<turnstile> tn \<triangleright> te2) \<and> te1 \<le> te2"
+        have ter: "\<exists> te2. (g2 \<turnstile> tn \<simeq> te2) \<and> te1 \<ge> te2"
           using ConditionalNode a b c d l no_encoding not_excluded_keep_type repDet singletonD
           by (metis IRNode.inject(6))
-        have "\<exists> fe2. (g2 \<turnstile> fn \<triangleright> fe2) \<and> fe1 \<le> fe2"
+        have "\<exists> fe2. (g2 \<turnstile> fn \<simeq> fe2) \<and> fe1 \<ge> fe2"
           using ConditionalNode a b c d l no_encoding not_excluded_keep_type repDet singletonD
           by (metis IRNode.inject(6))
-        then have "\<exists> ce2 te2 fe2. (g2 \<turnstile> n \<triangleright> ConditionalExpr ce2 te2 fe2) \<and> ConditionalExpr ce1 te1 fe1 \<le> ConditionalExpr ce2 te2 fe2"
+        then have "\<exists> ce2 te2 fe2. (g2 \<turnstile> n \<simeq> ConditionalExpr ce2 te2 fe2) \<and> ConditionalExpr ce1 te1 fe1 \<ge> ConditionalExpr ce2 te2 fe2"
           using ConditionalNode.prems l mono_conditional rep.ConditionalNode cer ter
           by (smt (verit) IRTreeEvalThms.mono_conditional)
         then show ?thesis
@@ -208,438 +208,438 @@ proof -
       qed
     next
       case (AbsNode n x xe1)
-      have k: "g1 \<turnstile> n \<triangleright> UnaryExpr UnaryAbs xe1" using f AbsNode
+      have k: "g1 \<turnstile> n \<simeq> UnaryExpr UnaryAbs xe1" using f AbsNode
         by (simp add: AbsNode.hyps(2) rep.AbsNode)
       obtain xn where l: "kind g1 n = AbsNode xn"
         using AbsNode.hyps(1) by blast
-      then have m: "g1 \<turnstile> xn \<triangleright> xe1"
+      then have m: "g1 \<turnstile> xn \<simeq> xe1"
         using AbsNode.hyps(1) AbsNode.hyps(2) by fastforce
       then show ?case
       proof (cases "xn = n'")
         case True
         then have n: "xe1 = e1'" using c m repDet by simp
-        then have ev: "g2 \<turnstile> n \<triangleright> UnaryExpr UnaryAbs e2'" using AbsNode.hyps(1) l m n
+        then have ev: "g2 \<turnstile> n \<simeq> UnaryExpr UnaryAbs e2'" using AbsNode.hyps(1) l m n
           using AbsNode.prems True d rep.AbsNode by simp
-        then have r: "UnaryExpr UnaryAbs e1' \<le> UnaryExpr UnaryAbs e2'"
+        then have r: "UnaryExpr UnaryAbs e1' \<ge> UnaryExpr UnaryAbs e2'"
           by (meson a mono_unary)
         then show ?thesis using ev r
           by (metis n)
       next
         case False
-        have "g1 \<turnstile> xn \<triangleright> xe1" using m by simp
-        have "\<exists> xe2. (g2 \<turnstile> xn \<triangleright> xe2) \<and> xe1 \<le> xe2"
+        have "g1 \<turnstile> xn \<simeq> xe1" using m by simp
+        have "\<exists> xe2. (g2 \<turnstile> xn \<simeq> xe2) \<and> xe1 \<ge> xe2"
           using AbsNode
           by (metis False IRNode.inject(1) b encodes_contains l not_excluded_keep_type not_in_g singleton_iff)
-        then have "\<exists> xe2. (g2 \<turnstile> n \<triangleright> UnaryExpr UnaryAbs xe2) \<and> UnaryExpr UnaryAbs xe1 \<le> UnaryExpr UnaryAbs xe2"
+        then have "\<exists> xe2. (g2 \<turnstile> n \<simeq> UnaryExpr UnaryAbs xe2) \<and> UnaryExpr UnaryAbs xe1 \<ge> UnaryExpr UnaryAbs xe2"
           by (metis AbsNode.prems l mono_unary rep.AbsNode)
         then show ?thesis
           by meson
       qed
     next
       case (NotNode n x xe1)
-      have k: "g1 \<turnstile> n \<triangleright> UnaryExpr UnaryNot xe1" using f NotNode
+      have k: "g1 \<turnstile> n \<simeq> UnaryExpr UnaryNot xe1" using f NotNode
         by (simp add: NotNode.hyps(2) rep.NotNode)
       obtain xn where l: "kind g1 n = NotNode xn"
         using NotNode.hyps(1) by blast
-      then have m: "g1 \<turnstile> xn \<triangleright> xe1"
+      then have m: "g1 \<turnstile> xn \<simeq> xe1"
         using NotNode.hyps(1) NotNode.hyps(2) by fastforce
       then show ?case
       proof (cases "xn = n'")
         case True
         then have n: "xe1 = e1'" using c m repDet by simp
-        then have ev: "g2 \<turnstile> n \<triangleright> UnaryExpr UnaryNot e2'" using NotNode.hyps(1) l m n
+        then have ev: "g2 \<turnstile> n \<simeq> UnaryExpr UnaryNot e2'" using NotNode.hyps(1) l m n
           using NotNode.prems True d rep.NotNode by simp
-        then have r: "UnaryExpr UnaryNot e1' \<le> UnaryExpr UnaryNot e2'"
+        then have r: "UnaryExpr UnaryNot e1' \<ge> UnaryExpr UnaryNot e2'"
           by (meson a mono_unary)
         then show ?thesis using ev r
           by (metis n)
       next
         case False
-        have "g1 \<turnstile> xn \<triangleright> xe1" using m by simp
-        have "\<exists> xe2. (g2 \<turnstile> xn \<triangleright> xe2) \<and> xe1 \<le> xe2"
+        have "g1 \<turnstile> xn \<simeq> xe1" using m by simp
+        have "\<exists> xe2. (g2 \<turnstile> xn \<simeq> xe2) \<and> xe1 \<ge> xe2"
           using NotNode
           by (metis False IRNode.inject(31) b l not_excluded_keep_type singletonD no_encoding)
-        then have "\<exists> xe2. (g2 \<turnstile> n \<triangleright> UnaryExpr UnaryNot xe2) \<and> UnaryExpr UnaryNot xe1 \<le> UnaryExpr UnaryNot xe2"
+        then have "\<exists> xe2. (g2 \<turnstile> n \<simeq> UnaryExpr UnaryNot xe2) \<and> UnaryExpr UnaryNot xe1 \<ge> UnaryExpr UnaryNot xe2"
           by (metis NotNode.prems l mono_unary rep.NotNode)
         then show ?thesis
           by meson
       qed
     next
       case (NegateNode n x xe1)
-      have k: "g1 \<turnstile> n \<triangleright> UnaryExpr UnaryNeg xe1" using f NegateNode
+      have k: "g1 \<turnstile> n \<simeq> UnaryExpr UnaryNeg xe1" using f NegateNode
         by (simp add: NegateNode.hyps(2) rep.NegateNode)
       obtain xn where l: "kind g1 n = NegateNode xn"
         using NegateNode.hyps(1) by blast
-      then have m: "g1 \<turnstile> xn \<triangleright> xe1"
+      then have m: "g1 \<turnstile> xn \<simeq> xe1"
         using NegateNode.hyps(1) NegateNode.hyps(2) by fastforce
       then show ?case
       proof (cases "xn = n'")
         case True
         then have n: "xe1 = e1'" using c m repDet by simp
-        then have ev: "g2 \<turnstile> n \<triangleright> UnaryExpr UnaryNeg e2'" using NegateNode.hyps(1) l m n
+        then have ev: "g2 \<turnstile> n \<simeq> UnaryExpr UnaryNeg e2'" using NegateNode.hyps(1) l m n
           using NegateNode.prems True d rep.NegateNode by simp
-        then have r: "UnaryExpr UnaryNeg e1' \<le> UnaryExpr UnaryNeg e2'"
+        then have r: "UnaryExpr UnaryNeg e1' \<ge> UnaryExpr UnaryNeg e2'"
           by (meson a mono_unary)
         then show ?thesis using ev r
           by (metis n)
       next
         case False
-        have "g1 \<turnstile> xn \<triangleright> xe1" using m by simp
-        have "\<exists> xe2. (g2 \<turnstile> xn \<triangleright> xe2) \<and> xe1 \<le> xe2"
+        have "g1 \<turnstile> xn \<simeq> xe1" using m by simp
+        have "\<exists> xe2. (g2 \<turnstile> xn \<simeq> xe2) \<and> xe1 \<ge> xe2"
           using NegateNode
           by (metis False IRNode.inject(28) b l not_excluded_keep_type singleton_iff no_encoding)
-        then have "\<exists> xe2. (g2 \<turnstile> n \<triangleright> UnaryExpr UnaryNeg xe2) \<and> UnaryExpr UnaryNeg xe1 \<le> UnaryExpr UnaryNeg xe2"
+        then have "\<exists> xe2. (g2 \<turnstile> n \<simeq> UnaryExpr UnaryNeg xe2) \<and> UnaryExpr UnaryNeg xe1 \<ge> UnaryExpr UnaryNeg xe2"
           by (metis NegateNode.prems l mono_unary rep.NegateNode)
         then show ?thesis
           by meson
       qed
     next
       case (LogicNegationNode n x xe1)
-      have k: "g1 \<turnstile> n \<triangleright> UnaryExpr UnaryLogicNegation xe1" using f LogicNegationNode
+      have k: "g1 \<turnstile> n \<simeq> UnaryExpr UnaryLogicNegation xe1" using f LogicNegationNode
         by (simp add: LogicNegationNode.hyps(2) rep.LogicNegationNode)
       obtain xn where l: "kind g1 n = LogicNegationNode xn"
         using LogicNegationNode.hyps(1) by blast
-      then have m: "g1 \<turnstile> xn \<triangleright> xe1"
+      then have m: "g1 \<turnstile> xn \<simeq> xe1"
         using LogicNegationNode.hyps(1) LogicNegationNode.hyps(2) by fastforce
       then show ?case
       proof (cases "xn = n'")
         case True
         then have n: "xe1 = e1'" using c m repDet by simp
-        then have ev: "g2 \<turnstile> n \<triangleright> UnaryExpr UnaryLogicNegation e2'" using LogicNegationNode.hyps(1) l m n
+        then have ev: "g2 \<turnstile> n \<simeq> UnaryExpr UnaryLogicNegation e2'" using LogicNegationNode.hyps(1) l m n
           using LogicNegationNode.prems True d rep.LogicNegationNode by simp
-        then have r: "UnaryExpr UnaryLogicNegation e1' \<le> UnaryExpr UnaryLogicNegation e2'"
+        then have r: "UnaryExpr UnaryLogicNegation e1' \<ge> UnaryExpr UnaryLogicNegation e2'"
           by (meson a mono_unary)
         then show ?thesis using ev r
           by (metis n)
       next
         case False
-        have "g1 \<turnstile> xn \<triangleright> xe1" using m by simp
-        have "\<exists> xe2. (g2 \<turnstile> xn \<triangleright> xe2) \<and> xe1 \<le> xe2"
+        have "g1 \<turnstile> xn \<simeq> xe1" using m by simp
+        have "\<exists> xe2. (g2 \<turnstile> xn \<simeq> xe2) \<and> xe1 \<ge> xe2"
           using LogicNegationNode
           by (metis False IRNode.inject(20) b encodes_contains ids_some l not_excluded_keep_type singleton_iff)
-        then have "\<exists> xe2. (g2 \<turnstile> n \<triangleright> UnaryExpr UnaryLogicNegation xe2) \<and> UnaryExpr UnaryLogicNegation xe1 \<le> UnaryExpr UnaryLogicNegation xe2"
+        then have "\<exists> xe2. (g2 \<turnstile> n \<simeq> UnaryExpr UnaryLogicNegation xe2) \<and> UnaryExpr UnaryLogicNegation xe1 \<ge> UnaryExpr UnaryLogicNegation xe2"
           by (metis LogicNegationNode.prems l mono_unary rep.LogicNegationNode)
         then show ?thesis
           by meson
       qed
     next
       case (AddNode n x y xe1 ye1)
-      have k: "g1 \<turnstile> n \<triangleright> BinaryExpr BinAdd xe1 ye1" using f AddNode
+      have k: "g1 \<turnstile> n \<simeq> BinaryExpr BinAdd xe1 ye1" using f AddNode
         by (simp add: AddNode.hyps(2) rep.AddNode)
       obtain xn yn where l: "kind g1 n = AddNode xn yn"
         using AddNode.hyps(1) by blast
-      then have mx: "g1 \<turnstile> xn \<triangleright> xe1"
+      then have mx: "g1 \<turnstile> xn \<simeq> xe1"
         using AddNode.hyps(1) AddNode.hyps(2) by fastforce
-      from l have my: "g1 \<turnstile> yn \<triangleright> ye1"
+      from l have my: "g1 \<turnstile> yn \<simeq> ye1"
         using AddNode.hyps(1) AddNode.hyps(3) by fastforce
       then show ?case
       proof -
-        have "g1 \<turnstile> xn \<triangleright> xe1" using mx by simp
-        have "g1 \<turnstile> yn \<triangleright> ye1" using my by simp
-        have xer: "\<exists> xe2. (g2 \<turnstile> xn \<triangleright> xe2) \<and> xe1 \<le> xe2"
+        have "g1 \<turnstile> xn \<simeq> xe1" using mx by simp
+        have "g1 \<turnstile> yn \<simeq> ye1" using my by simp
+        have xer: "\<exists> xe2. (g2 \<turnstile> xn \<simeq> xe2) \<and> xe1 \<ge> xe2"
           using AddNode
           by (metis IRNode.inject(2) a b c d l no_encoding not_excluded_keep_type repDet singletonD)
-        have "\<exists> ye2. (g2 \<turnstile> yn \<triangleright> ye2) \<and> ye1 \<le> ye2"
+        have "\<exists> ye2. (g2 \<turnstile> yn \<simeq> ye2) \<and> ye1 \<ge> ye2"
           using AddNode
           by (metis IRNode.inject(2) a b c d l no_encoding not_excluded_keep_type repDet singletonD)
-        then have "\<exists> xe2 ye2. (g2 \<turnstile> n \<triangleright> BinaryExpr BinAdd xe2 ye2) \<and> BinaryExpr BinAdd xe1 ye1 \<le> BinaryExpr BinAdd xe2 ye2"
+        then have "\<exists> xe2 ye2. (g2 \<turnstile> n \<simeq> BinaryExpr BinAdd xe2 ye2) \<and> BinaryExpr BinAdd xe1 ye1 \<ge> BinaryExpr BinAdd xe2 ye2"
           by (metis AddNode.prems l mono_binary rep.AddNode xer)
         then show ?thesis
           by meson
       qed
     next
       case (MulNode n x y xe1 ye1)
-      have k: "g1 \<turnstile> n \<triangleright> BinaryExpr BinMul xe1 ye1" using f MulNode
+      have k: "g1 \<turnstile> n \<simeq> BinaryExpr BinMul xe1 ye1" using f MulNode
         by (simp add: MulNode.hyps(2) rep.MulNode)
       obtain xn yn where l: "kind g1 n = MulNode xn yn"
         using MulNode.hyps(1) by blast
-      then have mx: "g1 \<turnstile> xn \<triangleright> xe1"
+      then have mx: "g1 \<turnstile> xn \<simeq> xe1"
         using MulNode.hyps(1) MulNode.hyps(2) by fastforce
-      from l have my: "g1 \<turnstile> yn \<triangleright> ye1"
+      from l have my: "g1 \<turnstile> yn \<simeq> ye1"
         using MulNode.hyps(1) MulNode.hyps(3) by fastforce
       then show ?case
       proof -
-        have "g1 \<turnstile> xn \<triangleright> xe1" using mx by simp
-        have "g1 \<turnstile> yn \<triangleright> ye1" using my by simp
-        have xer: "\<exists> xe2. (g2 \<turnstile> xn \<triangleright> xe2) \<and> xe1 \<le> xe2"
+        have "g1 \<turnstile> xn \<simeq> xe1" using mx by simp
+        have "g1 \<turnstile> yn \<simeq> ye1" using my by simp
+        have xer: "\<exists> xe2. (g2 \<turnstile> xn \<simeq> xe2) \<and> xe1 \<ge> xe2"
           using MulNode
           by (metis IRNode.inject(26) a b c d l no_encoding not_excluded_keep_type repDet singletonD)
-        have "\<exists> ye2. (g2 \<turnstile> yn \<triangleright> ye2) \<and> ye1 \<le> ye2"
+        have "\<exists> ye2. (g2 \<turnstile> yn \<simeq> ye2) \<and> ye1 \<ge> ye2"
           using MulNode
           by (metis IRNode.inject(26) a b c d l no_encoding not_excluded_keep_type repDet singletonD)
-        then have "\<exists> xe2 ye2. (g2 \<turnstile> n \<triangleright> BinaryExpr BinMul xe2 ye2) \<and> BinaryExpr BinMul xe1 ye1 \<le> BinaryExpr BinMul xe2 ye2"
+        then have "\<exists> xe2 ye2. (g2 \<turnstile> n \<simeq> BinaryExpr BinMul xe2 ye2) \<and> BinaryExpr BinMul xe1 ye1 \<ge> BinaryExpr BinMul xe2 ye2"
           by (metis MulNode.prems l mono_binary rep.MulNode xer)
         then show ?thesis
           by meson
       qed
     next
       case (SubNode n x y xe1 ye1)
-      have k: "g1 \<turnstile> n \<triangleright> BinaryExpr BinSub xe1 ye1" using f SubNode
+      have k: "g1 \<turnstile> n \<simeq> BinaryExpr BinSub xe1 ye1" using f SubNode
         by (simp add: SubNode.hyps(2) rep.SubNode)
       obtain xn yn where l: "kind g1 n = SubNode xn yn"
         using SubNode.hyps(1) by blast
-      then have mx: "g1 \<turnstile> xn \<triangleright> xe1"
+      then have mx: "g1 \<turnstile> xn \<simeq> xe1"
         using SubNode.hyps(1) SubNode.hyps(2) by fastforce
-      from l have my: "g1 \<turnstile> yn \<triangleright> ye1"
+      from l have my: "g1 \<turnstile> yn \<simeq> ye1"
         using SubNode.hyps(1) SubNode.hyps(3) by fastforce
       then show ?case
       proof -
-        have "g1 \<turnstile> xn \<triangleright> xe1" using mx by simp
-        have "g1 \<turnstile> yn \<triangleright> ye1" using my by simp
-        have xer: "\<exists> xe2. (g2 \<turnstile> xn \<triangleright> xe2) \<and> xe1 \<le> xe2"
+        have "g1 \<turnstile> xn \<simeq> xe1" using mx by simp
+        have "g1 \<turnstile> yn \<simeq> ye1" using my by simp
+        have xer: "\<exists> xe2. (g2 \<turnstile> xn \<simeq> xe2) \<and> xe1 \<ge> xe2"
           using SubNode
           using a b c d l no_encoding not_excluded_keep_type repDet singletonD
           by (metis IRNode.inject(42))
-        have "\<exists> ye2. (g2 \<turnstile> yn \<triangleright> ye2) \<and> ye1 \<le> ye2"
+        have "\<exists> ye2. (g2 \<turnstile> yn \<simeq> ye2) \<and> ye1 \<ge> ye2"
           using SubNode a b c d l no_encoding not_excluded_keep_type repDet singletonD
           by (metis IRNode.inject(42))
-        then have "\<exists> xe2 ye2. (g2 \<turnstile> n \<triangleright> BinaryExpr BinSub xe2 ye2) \<and> BinaryExpr BinSub xe1 ye1 \<le> BinaryExpr BinSub xe2 ye2"
+        then have "\<exists> xe2 ye2. (g2 \<turnstile> n \<simeq> BinaryExpr BinSub xe2 ye2) \<and> BinaryExpr BinSub xe1 ye1 \<ge> BinaryExpr BinSub xe2 ye2"
           by (metis SubNode.prems l mono_binary rep.SubNode xer)
         then show ?thesis
           by meson
       qed
     next
       case (AndNode n x y xe1 ye1)
-      have k: "g1 \<turnstile> n \<triangleright> BinaryExpr BinAnd xe1 ye1" using f AndNode
+      have k: "g1 \<turnstile> n \<simeq> BinaryExpr BinAnd xe1 ye1" using f AndNode
         by (simp add: AndNode.hyps(2) rep.AndNode)
       obtain xn yn where l: "kind g1 n = AndNode xn yn"
         using AndNode.hyps(1) by blast
-      then have mx: "g1 \<turnstile> xn \<triangleright> xe1"
+      then have mx: "g1 \<turnstile> xn \<simeq> xe1"
         using AndNode.hyps(1) AndNode.hyps(2) by fastforce
-      from l have my: "g1 \<turnstile> yn \<triangleright> ye1"
+      from l have my: "g1 \<turnstile> yn \<simeq> ye1"
         using AndNode.hyps(1) AndNode.hyps(3) by fastforce
       then show ?case
       proof -
-        have "g1 \<turnstile> xn \<triangleright> xe1" using mx by simp
-        have "g1 \<turnstile> yn \<triangleright> ye1" using my by simp
-        have xer: "\<exists> xe2. (g2 \<turnstile> xn \<triangleright> xe2) \<and> xe1 \<le> xe2"
+        have "g1 \<turnstile> xn \<simeq> xe1" using mx by simp
+        have "g1 \<turnstile> yn \<simeq> ye1" using my by simp
+        have xer: "\<exists> xe2. (g2 \<turnstile> xn \<simeq> xe2) \<and> xe1 \<ge> xe2"
           using AndNode
           using a b c d l no_encoding not_excluded_keep_type repDet singletonD
           by (metis IRNode.inject(3))
-        have "\<exists> ye2. (g2 \<turnstile> yn \<triangleright> ye2) \<and> ye1 \<le> ye2"
+        have "\<exists> ye2. (g2 \<turnstile> yn \<simeq> ye2) \<and> ye1 \<ge> ye2"
           using AndNode a b c d l no_encoding not_excluded_keep_type repDet singletonD
           by (metis IRNode.inject(3))
-        then have "\<exists> xe2 ye2. (g2 \<turnstile> n \<triangleright> BinaryExpr BinAnd xe2 ye2) \<and> BinaryExpr BinAnd xe1 ye1 \<le> BinaryExpr BinAnd xe2 ye2"
+        then have "\<exists> xe2 ye2. (g2 \<turnstile> n \<simeq> BinaryExpr BinAnd xe2 ye2) \<and> BinaryExpr BinAnd xe1 ye1 \<ge> BinaryExpr BinAnd xe2 ye2"
           by (metis AndNode.prems l mono_binary rep.AndNode xer)
         then show ?thesis
           by meson
       qed
     next
       case (OrNode n x y xe1 ye1)
-      have k: "g1 \<turnstile> n \<triangleright> BinaryExpr BinOr xe1 ye1" using f OrNode
+      have k: "g1 \<turnstile> n \<simeq> BinaryExpr BinOr xe1 ye1" using f OrNode
         by (simp add: OrNode.hyps(2) rep.OrNode)
       obtain xn yn where l: "kind g1 n = OrNode xn yn"
         using OrNode.hyps(1) by blast
-      then have mx: "g1 \<turnstile> xn \<triangleright> xe1"
+      then have mx: "g1 \<turnstile> xn \<simeq> xe1"
         using OrNode.hyps(1) OrNode.hyps(2) by fastforce
-      from l have my: "g1 \<turnstile> yn \<triangleright> ye1"
+      from l have my: "g1 \<turnstile> yn \<simeq> ye1"
         using OrNode.hyps(1) OrNode.hyps(3) by fastforce
       then show ?case
       proof -
-        have "g1 \<turnstile> xn \<triangleright> xe1" using mx by simp
-        have "g1 \<turnstile> yn \<triangleright> ye1" using my by simp
-        have xer: "\<exists> xe2. (g2 \<turnstile> xn \<triangleright> xe2) \<and> xe1 \<le> xe2"
+        have "g1 \<turnstile> xn \<simeq> xe1" using mx by simp
+        have "g1 \<turnstile> yn \<simeq> ye1" using my by simp
+        have xer: "\<exists> xe2. (g2 \<turnstile> xn \<simeq> xe2) \<and> xe1 \<ge> xe2"
           using OrNode
           using a b c d l no_encoding not_excluded_keep_type repDet singletonD
           by (metis IRNode.inject(32))
-        have "\<exists> ye2. (g2 \<turnstile> yn \<triangleright> ye2) \<and> ye1 \<le> ye2"
+        have "\<exists> ye2. (g2 \<turnstile> yn \<simeq> ye2) \<and> ye1 \<ge> ye2"
           using OrNode a b c d l no_encoding not_excluded_keep_type repDet singletonD
           by (metis IRNode.inject(32))
-        then have "\<exists> xe2 ye2. (g2 \<turnstile> n \<triangleright> BinaryExpr BinOr xe2 ye2) \<and> BinaryExpr BinOr xe1 ye1 \<le> BinaryExpr BinOr xe2 ye2"
+        then have "\<exists> xe2 ye2. (g2 \<turnstile> n \<simeq> BinaryExpr BinOr xe2 ye2) \<and> BinaryExpr BinOr xe1 ye1 \<ge> BinaryExpr BinOr xe2 ye2"
           by (metis OrNode.prems l mono_binary rep.OrNode xer)
         then show ?thesis
           by meson
       qed
     next
       case (XorNode n x y xe1 ye1)
-      have k: "g1 \<turnstile> n \<triangleright> BinaryExpr BinXor xe1 ye1" using f XorNode
+      have k: "g1 \<turnstile> n \<simeq> BinaryExpr BinXor xe1 ye1" using f XorNode
         by (simp add: XorNode.hyps(2) rep.XorNode)
       obtain xn yn where l: "kind g1 n = XorNode xn yn"
         using XorNode.hyps(1) by blast
-      then have mx: "g1 \<turnstile> xn \<triangleright> xe1"
+      then have mx: "g1 \<turnstile> xn \<simeq> xe1"
         using XorNode.hyps(1) XorNode.hyps(2) by fastforce
-      from l have my: "g1 \<turnstile> yn \<triangleright> ye1"
+      from l have my: "g1 \<turnstile> yn \<simeq> ye1"
         using XorNode.hyps(1) XorNode.hyps(3) by fastforce
       then show ?case
       proof -
-        have "g1 \<turnstile> xn \<triangleright> xe1" using mx by simp
-        have "g1 \<turnstile> yn \<triangleright> ye1" using my by simp
-        have xer: "\<exists> xe2. (g2 \<turnstile> xn \<triangleright> xe2) \<and> xe1 \<le> xe2"
+        have "g1 \<turnstile> xn \<simeq> xe1" using mx by simp
+        have "g1 \<turnstile> yn \<simeq> ye1" using my by simp
+        have xer: "\<exists> xe2. (g2 \<turnstile> xn \<simeq> xe2) \<and> xe1 \<ge> xe2"
           using XorNode
           using a b c d l no_encoding not_excluded_keep_type repDet singletonD
           by (metis IRNode.inject(46))
-        have "\<exists> ye2. (g2 \<turnstile> yn \<triangleright> ye2) \<and> ye1 \<le> ye2"
+        have "\<exists> ye2. (g2 \<turnstile> yn \<simeq> ye2) \<and> ye1 \<ge> ye2"
           using XorNode a b c d l no_encoding not_excluded_keep_type repDet singletonD
           by (metis IRNode.inject(46))
-        then have "\<exists> xe2 ye2. (g2 \<turnstile> n \<triangleright> BinaryExpr BinXor xe2 ye2) \<and> BinaryExpr BinXor xe1 ye1 \<le> BinaryExpr BinXor xe2 ye2"
+        then have "\<exists> xe2 ye2. (g2 \<turnstile> n \<simeq> BinaryExpr BinXor xe2 ye2) \<and> BinaryExpr BinXor xe1 ye1 \<ge> BinaryExpr BinXor xe2 ye2"
           by (metis XorNode.prems l mono_binary rep.XorNode xer)
         then show ?thesis
           by meson
       qed
     next
       case (IntegerBelowNode n x y xe1 ye1)
-      have k: "g1 \<turnstile> n \<triangleright> BinaryExpr BinIntegerBelow xe1 ye1" using f IntegerBelowNode
+      have k: "g1 \<turnstile> n \<simeq> BinaryExpr BinIntegerBelow xe1 ye1" using f IntegerBelowNode
         by (simp add: IntegerBelowNode.hyps(2) rep.IntegerBelowNode)
       obtain xn yn where l: "kind g1 n = IntegerBelowNode xn yn"
         using IntegerBelowNode.hyps(1) by blast
-      then have mx: "g1 \<turnstile> xn \<triangleright> xe1"
+      then have mx: "g1 \<turnstile> xn \<simeq> xe1"
         using IntegerBelowNode.hyps(1) IntegerBelowNode.hyps(2) by fastforce
-      from l have my: "g1 \<turnstile> yn \<triangleright> ye1"
+      from l have my: "g1 \<turnstile> yn \<simeq> ye1"
         using IntegerBelowNode.hyps(1) IntegerBelowNode.hyps(3) by fastforce
       then show ?case
       proof -
-        have "g1 \<turnstile> xn \<triangleright> xe1" using mx by simp
-        have "g1 \<turnstile> yn \<triangleright> ye1" using my by simp
-        have xer: "\<exists> xe2. (g2 \<turnstile> xn \<triangleright> xe2) \<and> xe1 \<le> xe2"
+        have "g1 \<turnstile> xn \<simeq> xe1" using mx by simp
+        have "g1 \<turnstile> yn \<simeq> ye1" using my by simp
+        have xer: "\<exists> xe2. (g2 \<turnstile> xn \<simeq> xe2) \<and> xe1 \<ge> xe2"
           using IntegerBelowNode
           using a b c d l no_encoding not_excluded_keep_type repDet singletonD
           by (metis IRNode.inject(12))
-        have "\<exists> ye2. (g2 \<turnstile> yn \<triangleright> ye2) \<and> ye1 \<le> ye2"
+        have "\<exists> ye2. (g2 \<turnstile> yn \<simeq> ye2) \<and> ye1 \<ge> ye2"
           using IntegerBelowNode a b c d l no_encoding not_excluded_keep_type repDet singletonD
           by (metis IRNode.inject(12))
-        then have "\<exists> xe2 ye2. (g2 \<turnstile> n \<triangleright> BinaryExpr BinIntegerBelow xe2 ye2) \<and> BinaryExpr BinIntegerBelow xe1 ye1 \<le> BinaryExpr BinIntegerBelow xe2 ye2"
+        then have "\<exists> xe2 ye2. (g2 \<turnstile> n \<simeq> BinaryExpr BinIntegerBelow xe2 ye2) \<and> BinaryExpr BinIntegerBelow xe1 ye1 \<ge> BinaryExpr BinIntegerBelow xe2 ye2"
           by (metis IntegerBelowNode.prems l mono_binary rep.IntegerBelowNode xer)
         then show ?thesis
           by meson
       qed
     next
       case (IntegerEqualsNode n x y xe1 ye1)
-      have k: "g1 \<turnstile> n \<triangleright> BinaryExpr BinIntegerEquals xe1 ye1" using f IntegerEqualsNode
+      have k: "g1 \<turnstile> n \<simeq> BinaryExpr BinIntegerEquals xe1 ye1" using f IntegerEqualsNode
         by (simp add: IntegerEqualsNode.hyps(2) rep.IntegerEqualsNode)
       obtain xn yn where l: "kind g1 n = IntegerEqualsNode xn yn"
         using IntegerEqualsNode.hyps(1) by blast
-      then have mx: "g1 \<turnstile> xn \<triangleright> xe1"
+      then have mx: "g1 \<turnstile> xn \<simeq> xe1"
         using IntegerEqualsNode.hyps(1) IntegerEqualsNode.hyps(2) by fastforce
-      from l have my: "g1 \<turnstile> yn \<triangleright> ye1"
+      from l have my: "g1 \<turnstile> yn \<simeq> ye1"
         using IntegerEqualsNode.hyps(1) IntegerEqualsNode.hyps(3) by fastforce
       then show ?case
       proof -
-        have "g1 \<turnstile> xn \<triangleright> xe1" using mx by simp
-        have "g1 \<turnstile> yn \<triangleright> ye1" using my by simp
-        have xer: "\<exists> xe2. (g2 \<turnstile> xn \<triangleright> xe2) \<and> xe1 \<le> xe2"
+        have "g1 \<turnstile> xn \<simeq> xe1" using mx by simp
+        have "g1 \<turnstile> yn \<simeq> ye1" using my by simp
+        have xer: "\<exists> xe2. (g2 \<turnstile> xn \<simeq> xe2) \<and> xe1 \<ge> xe2"
           using IntegerEqualsNode
           using a b c d l no_encoding not_excluded_keep_type repDet singletonD
           by (metis IRNode.inject(13))
-        have "\<exists> ye2. (g2 \<turnstile> yn \<triangleright> ye2) \<and> ye1 \<le> ye2"
+        have "\<exists> ye2. (g2 \<turnstile> yn \<simeq> ye2) \<and> ye1 \<ge> ye2"
           using IntegerEqualsNode a b c d l no_encoding not_excluded_keep_type repDet singletonD
           by (metis IRNode.inject(13))
-        then have "\<exists> xe2 ye2. (g2 \<turnstile> n \<triangleright> BinaryExpr BinIntegerEquals xe2 ye2) \<and> BinaryExpr BinIntegerEquals xe1 ye1 \<le> BinaryExpr BinIntegerEquals xe2 ye2"
+        then have "\<exists> xe2 ye2. (g2 \<turnstile> n \<simeq> BinaryExpr BinIntegerEquals xe2 ye2) \<and> BinaryExpr BinIntegerEquals xe1 ye1 \<ge> BinaryExpr BinIntegerEquals xe2 ye2"
           by (metis IntegerEqualsNode.prems l mono_binary rep.IntegerEqualsNode xer)
         then show ?thesis
           by meson
       qed
     next
       case (IntegerLessThanNode n x y xe1 ye1)
-      have k: "g1 \<turnstile> n \<triangleright> BinaryExpr BinIntegerLessThan xe1 ye1" using f IntegerLessThanNode
+      have k: "g1 \<turnstile> n \<simeq> BinaryExpr BinIntegerLessThan xe1 ye1" using f IntegerLessThanNode
         by (simp add: IntegerLessThanNode.hyps(2) rep.IntegerLessThanNode)
       obtain xn yn where l: "kind g1 n = IntegerLessThanNode xn yn"
         using IntegerLessThanNode.hyps(1) by blast
-      then have mx: "g1 \<turnstile> xn \<triangleright> xe1"
+      then have mx: "g1 \<turnstile> xn \<simeq> xe1"
         using IntegerLessThanNode.hyps(1) IntegerLessThanNode.hyps(2) by fastforce
-      from l have my: "g1 \<turnstile> yn \<triangleright> ye1"
+      from l have my: "g1 \<turnstile> yn \<simeq> ye1"
         using IntegerLessThanNode.hyps(1) IntegerLessThanNode.hyps(3) by fastforce
       then show ?case
       proof -
-        have "g1 \<turnstile> xn \<triangleright> xe1" using mx by simp
-        have "g1 \<turnstile> yn \<triangleright> ye1" using my by simp
-        have xer: "\<exists> xe2. (g2 \<turnstile> xn \<triangleright> xe2) \<and> xe1 \<le> xe2"
+        have "g1 \<turnstile> xn \<simeq> xe1" using mx by simp
+        have "g1 \<turnstile> yn \<simeq> ye1" using my by simp
+        have xer: "\<exists> xe2. (g2 \<turnstile> xn \<simeq> xe2) \<and> xe1 \<ge> xe2"
           using IntegerLessThanNode
           using a b c d l no_encoding not_excluded_keep_type repDet singletonD
           by (metis IRNode.inject(14))
-        have "\<exists> ye2. (g2 \<turnstile> yn \<triangleright> ye2) \<and> ye1 \<le> ye2"
+        have "\<exists> ye2. (g2 \<turnstile> yn \<simeq> ye2) \<and> ye1 \<ge> ye2"
           using IntegerLessThanNode a b c d l no_encoding not_excluded_keep_type repDet singletonD
           by (metis IRNode.inject(14))
-        then have "\<exists> xe2 ye2. (g2 \<turnstile> n \<triangleright> BinaryExpr BinIntegerLessThan xe2 ye2) \<and> BinaryExpr BinIntegerLessThan xe1 ye1 \<le> BinaryExpr BinIntegerLessThan xe2 ye2"
+        then have "\<exists> xe2 ye2. (g2 \<turnstile> n \<simeq> BinaryExpr BinIntegerLessThan xe2 ye2) \<and> BinaryExpr BinIntegerLessThan xe1 ye1 \<ge> BinaryExpr BinIntegerLessThan xe2 ye2"
           by (metis IntegerLessThanNode.prems l mono_binary rep.IntegerLessThanNode xer)
         then show ?thesis
           by meson
       qed
     next
       case (NarrowNode n inputBits resultBits x xe1)
-      have k: "g1 \<turnstile> n \<triangleright> UnaryExpr (UnaryNarrow inputBits resultBits) xe1" using f NarrowNode
+      have k: "g1 \<turnstile> n \<simeq> UnaryExpr (UnaryNarrow inputBits resultBits) xe1" using f NarrowNode
         by (simp add: NarrowNode.hyps(2) rep.NarrowNode)
       obtain xn where l: "kind g1 n = NarrowNode inputBits resultBits xn"
         using NarrowNode.hyps(1) by blast
-      then have m: "g1 \<turnstile> xn \<triangleright> xe1"
+      then have m: "g1 \<turnstile> xn \<simeq> xe1"
         using NarrowNode.hyps(1) NarrowNode.hyps(2)
         by auto
       then show ?case
       proof (cases "xn = n'")
         case True
         then have n: "xe1 = e1'" using c m repDet by simp
-        then have ev: "g2 \<turnstile> n \<triangleright> UnaryExpr (UnaryNarrow inputBits resultBits) e2'" using NarrowNode.hyps(1) l m n
+        then have ev: "g2 \<turnstile> n \<simeq> UnaryExpr (UnaryNarrow inputBits resultBits) e2'" using NarrowNode.hyps(1) l m n
           using NarrowNode.prems True d rep.NarrowNode by simp
-        then have r: "UnaryExpr (UnaryNarrow inputBits resultBits) e1' \<le> UnaryExpr (UnaryNarrow inputBits resultBits) e2'"
+        then have r: "UnaryExpr (UnaryNarrow inputBits resultBits) e1' \<ge> UnaryExpr (UnaryNarrow inputBits resultBits) e2'"
           by (meson a mono_unary)
         then show ?thesis using ev r
           by (metis n)
       next
         case False
-        have "g1 \<turnstile> xn \<triangleright> xe1" using m by simp
-        have "\<exists> xe2. (g2 \<turnstile> xn \<triangleright> xe2) \<and> xe1 \<le> xe2"
+        have "g1 \<turnstile> xn \<simeq> xe1" using m by simp
+        have "\<exists> xe2. (g2 \<turnstile> xn \<simeq> xe2) \<and> xe1 \<ge> xe2"
           using NarrowNode
           by (metis False IRNode.inject(27) b encodes_contains l not_excluded_keep_type not_in_g singleton_iff)
-        then have "\<exists> xe2. (g2 \<turnstile> n \<triangleright> UnaryExpr (UnaryNarrow inputBits resultBits) xe2) \<and> UnaryExpr (UnaryNarrow inputBits resultBits) xe1 \<le> UnaryExpr (UnaryNarrow inputBits resultBits) xe2"
+        then have "\<exists> xe2. (g2 \<turnstile> n \<simeq> UnaryExpr (UnaryNarrow inputBits resultBits) xe2) \<and> UnaryExpr (UnaryNarrow inputBits resultBits) xe1 \<ge> UnaryExpr (UnaryNarrow inputBits resultBits) xe2"
           by (metis NarrowNode.prems l mono_unary rep.NarrowNode)
         then show ?thesis
           by meson
       qed
     next
       case (SignExtendNode n inputBits resultBits x xe1)
-      have k: "g1 \<turnstile> n \<triangleright> UnaryExpr (UnarySignExtend inputBits resultBits) xe1" using f SignExtendNode
+      have k: "g1 \<turnstile> n \<simeq> UnaryExpr (UnarySignExtend inputBits resultBits) xe1" using f SignExtendNode
         by (simp add: SignExtendNode.hyps(2) rep.SignExtendNode)
       obtain xn where l: "kind g1 n = SignExtendNode inputBits resultBits xn"
         using SignExtendNode.hyps(1) by blast
-      then have m: "g1 \<turnstile> xn \<triangleright> xe1"
+      then have m: "g1 \<turnstile> xn \<simeq> xe1"
         using SignExtendNode.hyps(1) SignExtendNode.hyps(2)
         by auto
       then show ?case
       proof (cases "xn = n'")
         case True
         then have n: "xe1 = e1'" using c m repDet by simp
-        then have ev: "g2 \<turnstile> n \<triangleright> UnaryExpr (UnarySignExtend inputBits resultBits) e2'" using SignExtendNode.hyps(1) l m n
+        then have ev: "g2 \<turnstile> n \<simeq> UnaryExpr (UnarySignExtend inputBits resultBits) e2'" using SignExtendNode.hyps(1) l m n
           using SignExtendNode.prems True d rep.SignExtendNode by simp
-        then have r: "UnaryExpr (UnarySignExtend inputBits resultBits) e1' \<le> UnaryExpr (UnarySignExtend inputBits resultBits) e2'"
+        then have r: "UnaryExpr (UnarySignExtend inputBits resultBits) e1' \<ge> UnaryExpr (UnarySignExtend inputBits resultBits) e2'"
           by (meson a mono_unary)
         then show ?thesis using ev r
           by (metis n)
       next
         case False
-        have "g1 \<turnstile> xn \<triangleright> xe1" using m by simp
-        have "\<exists> xe2. (g2 \<turnstile> xn \<triangleright> xe2) \<and> xe1 \<le> xe2"
+        have "g1 \<turnstile> xn \<simeq> xe1" using m by simp
+        have "\<exists> xe2. (g2 \<turnstile> xn \<simeq> xe2) \<and> xe1 \<ge> xe2"
           using SignExtendNode
           by (metis False IRNode.inject(37) b encodes_contains l not_excluded_keep_type not_in_g singleton_iff)
-        then have "\<exists> xe2. (g2 \<turnstile> n \<triangleright> UnaryExpr (UnarySignExtend inputBits resultBits) xe2) \<and> UnaryExpr (UnarySignExtend inputBits resultBits) xe1 \<le> UnaryExpr (UnarySignExtend inputBits resultBits) xe2"
+        then have "\<exists> xe2. (g2 \<turnstile> n \<simeq> UnaryExpr (UnarySignExtend inputBits resultBits) xe2) \<and> UnaryExpr (UnarySignExtend inputBits resultBits) xe1 \<ge> UnaryExpr (UnarySignExtend inputBits resultBits) xe2"
           by (metis SignExtendNode.prems l mono_unary rep.SignExtendNode)
         then show ?thesis
           by meson
       qed
     next
       case (ZeroExtendNode n inputBits resultBits x xe1)
-      have k: "g1 \<turnstile> n \<triangleright> UnaryExpr (UnaryZeroExtend inputBits resultBits) xe1" using f ZeroExtendNode
+      have k: "g1 \<turnstile> n \<simeq> UnaryExpr (UnaryZeroExtend inputBits resultBits) xe1" using f ZeroExtendNode
         by (simp add: ZeroExtendNode.hyps(2) rep.ZeroExtendNode)
       obtain xn where l: "kind g1 n = ZeroExtendNode inputBits resultBits xn"
         using ZeroExtendNode.hyps(1) by blast
-      then have m: "g1 \<turnstile> xn \<triangleright> xe1"
+      then have m: "g1 \<turnstile> xn \<simeq> xe1"
         using ZeroExtendNode.hyps(1) ZeroExtendNode.hyps(2)
         by auto
       then show ?case
       proof (cases "xn = n'")
         case True
         then have n: "xe1 = e1'" using c m repDet by simp
-        then have ev: "g2 \<turnstile> n \<triangleright> UnaryExpr (UnaryZeroExtend inputBits resultBits) e2'" using ZeroExtendNode.hyps(1) l m n
+        then have ev: "g2 \<turnstile> n \<simeq> UnaryExpr (UnaryZeroExtend inputBits resultBits) e2'" using ZeroExtendNode.hyps(1) l m n
           using ZeroExtendNode.prems True d rep.ZeroExtendNode by simp
-        then have r: "UnaryExpr (UnaryZeroExtend inputBits resultBits) e1' \<le> UnaryExpr (UnaryZeroExtend inputBits resultBits) e2'"
+        then have r: "UnaryExpr (UnaryZeroExtend inputBits resultBits) e1' \<ge> UnaryExpr (UnaryZeroExtend inputBits resultBits) e2'"
           by (meson a mono_unary)
         then show ?thesis using ev r
           by (metis n)
       next
         case False
-        have "g1 \<turnstile> xn \<triangleright> xe1" using m by simp
-        have "\<exists> xe2. (g2 \<turnstile> xn \<triangleright> xe2) \<and> xe1 \<le> xe2"
+        have "g1 \<turnstile> xn \<simeq> xe1" using m by simp
+        have "\<exists> xe2. (g2 \<turnstile> xn \<simeq> xe2) \<and> xe1 \<ge> xe2"
           using ZeroExtendNode
           by (metis False IRNode.inject(47) b encodes_contains l not_excluded_keep_type not_in_g singleton_iff)
-        then have "\<exists> xe2. (g2 \<turnstile> n \<triangleright> UnaryExpr (UnaryZeroExtend inputBits resultBits) xe2) \<and> UnaryExpr (UnaryZeroExtend inputBits resultBits) xe1 \<le> UnaryExpr (UnaryZeroExtend inputBits resultBits) xe2"
+        then have "\<exists> xe2. (g2 \<turnstile> n \<simeq> UnaryExpr (UnaryZeroExtend inputBits resultBits) xe2) \<and> UnaryExpr (UnaryZeroExtend inputBits resultBits) xe1 \<ge> UnaryExpr (UnaryZeroExtend inputBits resultBits) xe2"
           by (metis ZeroExtendNode.prems l mono_unary rep.ZeroExtendNode)
         then show ?thesis
           by meson
@@ -654,33 +654,33 @@ qed
 
 (*
         case (UnaryExpr op xe1)
-        from UnaryExpr have k: "g1 \<turnstile> n \<triangleright> UnaryExpr op xe1" using f by blast
+        from UnaryExpr have k: "g1 \<turnstile> n \<simeq> UnaryExpr op xe1" using f by blast
         have "\<not>(is_convert_node (kind g1 n))"
           using hack encodes_contains ids_some
           using e by blast
         then obtain xn where l: "embed_expr (kind g1 n) = ExprUnaryNode op xn"
           using k using unary_embed
           by blast
-        then have kk: "g1 \<turnstile> xn \<triangleright> xe1"
+        then have kk: "g1 \<turnstile> xn \<simeq> xe1"
           using repDet k equal_embedded_x by blast
         then show ?thesis
         proof (cases "xn = n'")
           case True
           then have n: "xe1 = e1'" using c UnaryExpr repDet l
             using kk by presburger
-          have r: "UnaryExpr op e1' \<le> UnaryExpr op e2'"
+          have r: "UnaryExpr op e1' \<ge> UnaryExpr op e2'"
             using a mono_unary by simp
-          have "g2 \<turnstile> n \<triangleright> UnaryExpr op e2'" using i k UnaryExpr n d True
+          have "g2 \<turnstile> n \<simeq> UnaryExpr op e2'" using i k UnaryExpr n d True
             using blah
             using l by presburger
           then show ?thesis
             using r UnaryExpr n by blast 
         next
           case False
-          then have "g1 \<turnstile> xn \<triangleright> xe1" using UnaryExpr
+          then have "g1 \<turnstile> xn \<simeq> xe1" using UnaryExpr
             by (simp add: kk)
-          then have "\<exists> xe2. (g2 \<turnstile> xn \<triangleright> xe2) \<and> xe1 \<le> xe2" sorry
-          then have "\<exists> xe2. (g2 \<turnstile> n \<triangleright> UnaryExpr op xe2) \<and> UnaryExpr op xe1 \<le> UnaryExpr op xe2"
+          then have "\<exists> xe2. (g2 \<turnstile> xn \<simeq> xe2) \<and> xe1 \<ge> xe2" sorry
+          then have "\<exists> xe2. (g2 \<turnstile> n \<simeq> UnaryExpr op xe2) \<and> UnaryExpr op xe1 \<ge> UnaryExpr op xe2"
             by (metis blah i l mono_unary)
           then show ?thesis
             using UnaryExpr by blast
@@ -707,7 +707,7 @@ qed
 
 (*
 lemma graph_semantics_preservation:
-  "e1 \<le> e2 \<and> (g1 \<turnstile> n \<triangleright> e1) \<and> (g2 \<turnstile> n \<triangleright> e2) \<and> (({n} \<unlhd> as_set g1) \<subseteq> as_set g2) \<Longrightarrow>
+  "e1 \<ge> e2 \<and> (g1 \<turnstile> n \<simeq> e1) \<and> (g2 \<turnstile> n \<simeq> e2) \<and> (({n} \<unlhd> as_set g1) \<subseteq> as_set g2) \<Longrightarrow>
      graph_refinement g1 g2" (is "?asm \<Longrightarrow> ?con")
 proof (cases "n \<in> ids g1")
   case True
@@ -718,7 +718,7 @@ proof (cases "n \<in> ids g1")
     fix n1 m p v
     assume a0: "n1 \<in> ids g1"
     assume a1: "([g1,m,p] \<turnstile> n1 \<mapsto> v)"
-    obtain e1 where "g1 \<turnstile> n1 \<triangleright> e1"
+    obtain e1 where "g1 \<turnstile> n1 \<simeq> e1"
       using a1 encodeeval_def by auto
     have same: "n1 \<notin> {n} \<Longrightarrow> kind g1 n1 = kind g2 n1 \<and> stamp g1 n1 = stamp g2 n1"
       using a a0 unfolding as_set_def domain_subtraction_def
@@ -737,7 +737,7 @@ next
     fix n m p v
     assume a0: "n \<in> ids g1"
     assume a1: "([g1,m,p] \<turnstile> n \<mapsto> v)"
-    have "\<not>(\<exists>e. (g1 \<turnstile> n \<triangleright> e))"
+    have "\<not>(\<exists>e. (g1 \<turnstile> n \<simeq> e))"
       using no_encoding
       by (meson False a)
     then show "([g2,m,p] \<turnstile> n \<mapsto> v)" using a0 a1 a unfolding encodeeval_def
@@ -749,13 +749,13 @@ qed
 
 definition maximal_sharing:
   "maximal_sharing g = (\<forall> n1 n2 . n1 \<in> ids g \<and> n2 \<in> ids g \<longrightarrow> 
-      (\<forall> e. (g \<turnstile> n1 \<triangleright> e) \<and> (g \<turnstile> n2 \<triangleright> e) \<longrightarrow> n1 = n2))"
+      (\<forall> e. (g \<turnstile> n1 \<simeq> e) \<and> (g \<turnstile> n2 \<simeq> e) \<longrightarrow> n1 = n2))"
 
 lemma tree_to_graph_rewriting:
-  "e1 \<le> e2 
-  \<and> (g1 \<turnstile> n \<triangleright> e1) \<and> maximal_sharing g1
+  "e1 \<ge> e2 
+  \<and> (g1 \<turnstile> n \<simeq> e1) \<and> maximal_sharing g1
   \<and> ({n} \<unlhd> as_set g1) \<subseteq> as_set g2 
-  \<and> (g2 \<turnstile> n \<triangleright> e2) \<and> maximal_sharing g2
+  \<and> (g2 \<turnstile> n \<simeq> e2) \<and> maximal_sharing g2
   \<Longrightarrow> graph_refinement g1 g2"
   using graph_semantics_preservation
   by auto
@@ -764,19 +764,19 @@ declare [[simp_trace]]
 lemma equal_refines:
   fixes e1 e2 :: IRExpr
   assumes "e1 = e2"
-  shows "e1 \<le> e2"
+  shows "e1 \<ge> e2"
   using assms
   by simp
 declare [[simp_trace=false]]
 
 inductive_cases UnaryRepE[elim!]:\<^marker>\<open>tag invisible\<close>
-  "g \<turnstile> n \<triangleright> (UnaryExpr op xe)"
+  "g \<turnstile> n \<simeq> (UnaryExpr op xe)"
 inductive_cases BinaryRepE[elim!]:\<^marker>\<open>tag invisible\<close>
-  "g \<turnstile> n \<triangleright> (BinaryExpr op xe ye)"
+  "g \<turnstile> n \<simeq> (BinaryExpr op xe ye)"
 
 lemma subset_implies_evals:
   assumes "as_set g1 \<subseteq> as_set g2"
-  shows "(g1 \<turnstile> n \<triangleright> e) \<Longrightarrow> (g2 \<turnstile> n \<triangleright> e)"
+  shows "(g1 \<turnstile> n \<simeq> e) \<Longrightarrow> (g2 \<turnstile> n \<simeq> e)"
 proof (induction e arbitrary: n)
   case (UnaryExpr op e)
   then have "n \<in> ids g1"
@@ -851,9 +851,9 @@ proof -
     proof -
       fix n e1
       assume 1:"n \<in> ids g1"
-      assume 2:"g1 \<turnstile> n \<triangleright> e1"
+      assume 2:"g1 \<turnstile> n \<simeq> e1"
   
-      show "\<exists>e2. (g2 \<turnstile> n \<triangleright> e2) \<and> e1 \<le> e2"
+      show "\<exists>e2. (g2 \<turnstile> n \<simeq> e2) \<and> e1 \<ge> e2"
         using assms 1 2 using subset_implies_evals
         by (meson equal_refines)
     qed
@@ -861,9 +861,9 @@ qed
 
 
 lemma graph_construction:
-  "e1 \<le> e2
+  "e1 \<ge> e2
   \<and> as_set g1 \<subseteq> as_set g2 \<and> maximal_sharing g1
-  \<and> (g2 \<turnstile> n \<triangleright> e2) \<and> maximal_sharing g2
+  \<and> (g2 \<turnstile> n \<simeq> e2) \<and> maximal_sharing g2
   \<Longrightarrow> graph_refinement g1 g2"
   using subset_refines
   by blast
