Semantics/IRStepObj.thy
@@ -78,7 +78,7 @@ inductive step :: "IRGraph \<Rightarrow> Params \<Rightarrow> (ID \<times> MapSt
 
   IfNode:
   "\<lbrakk>kind g nid = (IfNode cond tb fb);
-    g \<turnstile> cond \<triangleright> condE; 
+    g \<turnstile> cond \<simeq> condE; 
     [m, p] \<turnstile> condE \<mapsto> val;
     nid' = (if val_to_bool val then tb else fb)\<rbrakk>
     \<Longrightarrow> g, p \<turnstile> (nid, m, h) \<rightarrow> (nid', m, h)" |  
@@ -91,7 +91,7 @@ inductive step :: "IRGraph \<Rightarrow> Params \<Rightarrow> (ID \<times> MapSt
     i = find_index nid (inputs_of (kind g merge));
     phis = (phi_list g merge);
     inps = (phi_inputs g i phis);
-    g \<turnstile> inps \<triangleright>\<^sub>L inpsE;
+    g \<turnstile> inps \<simeq>\<^sub>L inpsE;
     [m, p] \<turnstile> inpsE \<mapsto>\<^sub>L vs;
 
     m' = set_phis phis vs m\<rbrakk>
@@ -106,7 +106,7 @@ inductive step :: "IRGraph \<Rightarrow> Params \<Rightarrow> (ID \<times> MapSt
 
   LoadFieldNode:
     "\<lbrakk>kind g nid = (LoadFieldNode nid f (Some obj) nid');
-      g \<turnstile> obj \<triangleright> objE; 
+      g \<turnstile> obj \<simeq> objE; 
       [m, p] \<turnstile> objE \<mapsto> ObjRef ref;
       h_load_field f ref h = v;
       m' = m(nid := v)\<rbrakk> 
@@ -114,8 +114,8 @@ inductive step :: "IRGraph \<Rightarrow> Params \<Rightarrow> (ID \<times> MapSt
 
   SignedDivNode:
     "\<lbrakk>kind g nid = (SignedDivNode nid x y zero sb nxt);
-      g \<turnstile> x \<triangleright> xe; 
-      g \<turnstile> y \<triangleright> ye; 
+      g \<turnstile> x \<simeq> xe; 
+      g \<turnstile> y \<simeq> ye; 
       [m, p] \<turnstile> xe \<mapsto> v1;
       [m, p] \<turnstile> ye \<mapsto> v2;
       v = (intval_div v1 v2);
@@ -124,8 +124,8 @@ inductive step :: "IRGraph \<Rightarrow> Params \<Rightarrow> (ID \<times> MapSt
 
   SignedRemNode:
     "\<lbrakk>kind g nid = (SignedRemNode nid x y zero sb nxt);
-      g \<turnstile> x \<triangleright> xe; 
-      g \<turnstile> y \<triangleright> ye; 
+      g \<turnstile> x \<simeq> xe; 
+      g \<turnstile> y \<simeq> ye; 
       [m, p] \<turnstile> xe \<mapsto> v1;
       [m, p] \<turnstile> ye \<mapsto> v2;
       v = (intval_mod v1 v2);
@@ -140,8 +140,8 @@ inductive step :: "IRGraph \<Rightarrow> Params \<Rightarrow> (ID \<times> MapSt
 
   StoreFieldNode:
     "\<lbrakk>kind g nid = (StoreFieldNode nid f newval _ (Some obj) nid');
-      g \<turnstile> newval \<triangleright> newvalE;
-      g \<turnstile> obj \<triangleright> objE; 
+      g \<turnstile> newval \<simeq> newvalE;
+      g \<turnstile> obj \<simeq> objE; 
       [m, p] \<turnstile> newvalE \<mapsto> val;
       [m, p] \<turnstile> objE \<mapsto> ObjRef ref;
       h' = h_store_field f ref val h;
@@ -150,7 +150,7 @@ inductive step :: "IRGraph \<Rightarrow> Params \<Rightarrow> (ID \<times> MapSt
 
   StaticStoreFieldNode:
     "\<lbrakk>kind g nid = (StoreFieldNode nid f newval _ None nid');
-      g \<turnstile> newval \<triangleright> newvalE; 
+      g \<turnstile> newval \<simeq> newvalE; 
       [m, p] \<turnstile> newvalE \<mapsto> val;
       h' = h_store_field f None val h;
       m' =  m(nid := val)\<rbrakk> 
@@ -179,13 +179,13 @@ inductive step_top :: "Program \<Rightarrow> (IRGraph \<times> ID \<times> MapSt
     kind g callTarget = (MethodCallTargetNode targetMethod arguments);
     Some targetGraph = P targetMethod;
     m' = new_map_state;
-    g \<turnstile> arguments \<triangleright>\<^sub>L argsE;
+    g \<turnstile> arguments \<simeq>\<^sub>L argsE;
     [m, p] \<turnstile> argsE  \<mapsto>\<^sub>L p'\<rbrakk>
     \<Longrightarrow> P \<turnstile> ((g,nid,m,p)#stk, h) \<longrightarrow> ((targetGraph,0,m',p')#(g,nid,m,p)#stk, h)" |
 
   ReturnNode:
   "\<lbrakk>kind g nid = (ReturnNode (Some expr) _);
-    g \<turnstile> expr \<triangleright> e;
+    g \<turnstile> expr \<simeq> e;
     [m, p] \<turnstile> e \<mapsto> v;
 
     cm' = cm(cnid := v);
@@ -202,7 +202,7 @@ inductive step_top :: "Program \<Rightarrow> (IRGraph \<times> ID \<times> MapSt
   UnwindNode:
   "\<lbrakk>kind g nid = (UnwindNode exception);
 
-    g \<turnstile> exception \<triangleright> exceptionE;
+    g \<turnstile> exception \<simeq> exceptionE;
     [m, p] \<turnstile> exceptionE \<mapsto> e;
      
     kind cg cnid = (InvokeWithExceptionNode _ _ _ _ _ _ exEdge);
